Weidenbach_Book/IsaSAT_Setup_LLVM.thy
@@ -1,0 +1,431 @@
+theory IsaSAT_Setup_LLVM
+  imports IsaSAT_Setup IsaSAT_Watch_List_LLVM IsaSAT_Lookup_Conflict_LLVM
+    IsaSAT_Clauses_LLVM LBD_LLVM
+begin
+
+find_in_thms of_nat in sepref_fr_rules  
+
+(* TODO: Move *)  
+sepref_register of_nat
+lemma of_nat_refine[sepref_import_param]: 
+  "(id,of_nat) \<in> unat_rel' TYPE('a::len) \<rightarrow> word_rel"
+  by (auto simp: unat_rel_def unat.rel_def in_br_conv)
+
+context fixes a::num begin  
+  sepref_register 
+    "numeral a :: _ word"  
+    "0 :: _ word"
+    "1 :: _ word"
+
+  lemma word_numeral_param[sepref_import_param]:
+    "(PR_CONST (numeral a),PR_CONST (numeral a)) \<in> word_rel"  
+    "(0,0)\<in>word_rel"
+    "(1,1)\<in>word_rel"
+    by auto
+        
+end
+ 
+
+
+
+(* TODO: Move *)  
+context begin
+  interpretation llvm_prim_arith_setup .
+
+    
+  definition [llvm_inline]: "unat_unat_upcast TYPE('a::len) x \<equiv> ll_zext x TYPE('a word)"
+  definition [llvm_inline]: "unat_unat_downcast TYPE('a::len) x \<equiv> ll_trunc x TYPE('a word)"
+
+   lemma unat_unat_upcast_rule[vcg_rules]:
+    "llvm_htriple 
+      (\<up>(is_up' UCAST('small \<rightarrow> 'big)) ** \<upharpoonleft>unat.assn n (ni::'small::len word)) 
+      (unat_unat_upcast TYPE('big::len) ni) 
+      (\<lambda>r. \<upharpoonleft>unat.assn n r)"
+    unfolding unat.assn_def snat.assn_def unat_unat_upcast_def
+    apply vcg'
+    apply (auto simp: snat_invar_def snat_eq_unat(2) unat_ucast_upcast)
+    done
+
+  lemma unat_unat_downcast_rule[vcg_rules]:
+    "llvm_htriple 
+      (\<up>(is_down' UCAST('big \<rightarrow> 'small)) ** \<upharpoonleft>unat.assn n (ni::'big::len word) ** \<up>(n<max_unat LENGTH('small))) 
+      (unat_unat_downcast TYPE('small::len) ni) 
+      (\<lambda>r. \<upharpoonleft>unat.assn n r)"
+    unfolding unat.assn_def unat.assn_def unat_unat_downcast_def
+    apply vcg'
+    apply (auto simp: snat_invar_def snat_eq_unat(2) max_unat_def)
+    by (metis ucast_nat_def unat_of_nat_eq)
+
+end
+
+(* TODO: Move *)  
+
+context fixes T :: "'a::len itself" begin
+  definition [simp]: "unat_unat_upcast_aux \<equiv> let _=TYPE('a) in id::nat\<Rightarrow>nat"
+
+  sepref_decl_op unat_unat_upcast: "unat_unat_upcast_aux" :: "nat_rel \<rightarrow> nat_rel" .
+end  
+
+context fixes T :: "'a::len itself" begin
+  definition [simp]: "unat_unat_downcast_aux \<equiv> let _=TYPE('a) in id::nat\<Rightarrow>nat"
+
+  sepref_decl_op unat_unat_downcast: "unat_unat_downcast_aux" :: "nat_rel \<rightarrow> nat_rel" .
+end
+lemma annot_unat_unat_upcast: "x = op_unat_unat_upcast TYPE('l::len) x" by simp 
+lemma annot_unat_unat_downcast: "x = op_unat_unat_downcast TYPE('l::len) x" by simp 
+
+
+term unat_unat_upcast
+
+context fixes BIG :: "'big::len" and SMALL :: "'small::len" begin  
+  lemma unat_unat_upcast_refine: 
+    "(unat_unat_upcast TYPE('big), PR_CONST (mop_unat_unat_upcast TYPE('big))) \<in> [\<lambda>_. is_up' UCAST('small \<rightarrow> 'big)]\<^sub>a (unat_assn' TYPE('small::len))\<^sup>k \<rightarrow> unat_assn"
+    supply [simp] = in_unat_rel_conv_assn
+    apply sepref_to_hoare
+    apply simp
+    by vcg'
+  
+  sepref_decl_impl (ismop) unat_unat_upcast_refine fixes 'big 'small by simp
+  
+  lemma unat_unat_downcast_refine: 
+    "(unat_unat_downcast TYPE('small), PR_CONST (mop_unat_unat_downcast TYPE('small))) 
+      \<in> [\<lambda>x. is_down' UCAST('big \<rightarrow> 'small) \<and> x<max_unat LENGTH('small)]\<^sub>a (unat_assn' TYPE('big::len))\<^sup>k \<rightarrow> unat_assn"
+    supply [simp] = in_unat_rel_conv_assn
+    apply sepref_to_hoare
+    apply simp
+    by vcg'
+  
+  sepref_decl_impl (ismop) unat_unat_downcast_refine fixes 'big 'small by simp
+end
+
+(* TODO: Setup llvm_inlines for these! *)
+definition word_shl :: "'a::len word \<Rightarrow> 'a word \<Rightarrow> 'a word" where "word_shl a b \<equiv> a << unat b"
+definition word_lshr :: "'a::len word \<Rightarrow> 'a word \<Rightarrow> 'a word" where "word_lshr a b \<equiv> a >> unat b"
+definition word_ashr :: "'a::len word \<Rightarrow> 'a word \<Rightarrow> 'a word" where "word_ashr a b \<equiv> a >>> unat b"
+
+
+(* TODO: Move *)  
+sepref_register 
+  shl_word: "(<<):: _ word \<Rightarrow> _"  
+  lshr_word: "(>>):: _ word \<Rightarrow> _"  
+  ashr_word: "(>>>):: _ word \<Rightarrow> _"  
+  
+lemma word_param_shift_imports[sepref_import_param]:
+  "(word_shl,(<<)::'a::len word \<Rightarrow> _) \<in> word_rel \<rightarrow> unat_rel \<rightarrow> word_rel"
+  "(word_lshr,(>>)::'a::len word \<Rightarrow> _) \<in> word_rel \<rightarrow> unat_rel \<rightarrow> word_rel"
+  "(word_ashr,(>>>)::'a::len word \<Rightarrow> _) \<in> word_rel \<rightarrow> unat_rel \<rightarrow> word_rel"
+  unfolding unat_rel_def unat.rel_def word_shl_def word_lshr_def word_ashr_def
+  by (auto simp: in_br_conv)
+
+(*TODO Move*)
+abbreviation "word32_rel \<equiv> word_rel :: (32 word \<times> _) set"
+abbreviation "word64_rel \<equiv> word_rel :: (64 word \<times> _) set"
+abbreviation "word32_assn \<equiv> word_assn :: 32 word \<Rightarrow> _"
+abbreviation "word64_assn \<equiv> word_assn :: 64 word \<Rightarrow> _"
+
+abbreviation stats_rel :: \<open>(stats \<times> stats) set\<close> where
+  \<open>stats_rel \<equiv> word64_rel \<times>\<^sub>r word64_rel \<times>\<^sub>r word64_rel \<times>\<^sub>r word64_rel \<times>\<^sub>r word64_rel
+     \<times>\<^sub>r word64_rel \<times>\<^sub>r word64_rel \<times>\<^sub>r word64_rel\<close>
+
+abbreviation ema_rel :: \<open>(ema\<times>ema) set\<close> where
+  \<open>ema_rel \<equiv> word64_rel \<times>\<^sub>r word64_rel \<times>\<^sub>r word64_rel \<times>\<^sub>r word64_rel \<times>\<^sub>r word64_rel\<close>
+     
+abbreviation ema_assn :: \<open>ema \<Rightarrow> ema \<Rightarrow> assn\<close> where
+  \<open>ema_assn \<equiv> word64_assn *a word64_assn *a word64_assn *a word64_assn *a word64_assn\<close>
+
+abbreviation stats_assn :: \<open>stats \<Rightarrow> stats \<Rightarrow> assn\<close> where
+  \<open>stats_assn \<equiv> word64_assn *a word64_assn *a word64_assn *a ema_assn\<close>
+  
+  
+lemma [sepref_import_param]: 
+  "(ema_get_value, ema_get_value) \<in> ema_rel \<rightarrow> word64_rel" 
+  "(ema_bitshifting,ema_bitshifting) \<in> word64_rel"
+  "(ema_reinit,ema_reinit) \<in> ema_rel \<rightarrow> ema_rel"
+  "(ema_init,ema_init) \<in> word_rel \<rightarrow> ema_rel"
+  by auto
+
+
+
+sepref_definition ema_update_impl is "uncurry (RETURN oo ema_update)"  
+  :: "uint32_nat_assn\<^sup>k *\<^sub>a ema_assn\<^sup>k \<rightarrow>\<^sub>a ema_assn"
+  unfolding ema_update_def
+  apply (rewrite at \<open>let _ = of_nat \<hole> * _ in _\<close> annot_unat_unat_upcast[where 'l = 64])
+  apply (rewrite at \<open>let _=_ + _; _=\<hole> in _\<close> fold_COPY)
+  (* TODO: The let x=y seems to be inlined, making necessary this COPY! Is this behaviour correct? *)
+  apply (annot_unat_const "TYPE(64)")
+  supply [[goals_limit = 1]]
+  supply [simp] = max_unat_def
+  by sepref
+lemmas [sepref_fr_rules] = ema_update_impl.refine
+  
+    
+  
+lemma [sepref_import_param]:
+  "(incr_propagation,incr_propagation) \<in> stats_rel \<rightarrow> stats_rel" 
+  "(incr_conflict,incr_conflict) \<in> stats_rel \<rightarrow> stats_rel" 
+  "(incr_decision,incr_decision) \<in> stats_rel \<rightarrow> stats_rel" 
+  "(incr_restart,incr_restart) \<in> stats_rel \<rightarrow> stats_rel" 
+  "(incr_lrestart,incr_lrestart) \<in> stats_rel \<rightarrow> stats_rel" 
+  "(incr_uset,incr_uset) \<in> stats_rel \<rightarrow> stats_rel" 
+  "(incr_GC,incr_GC) \<in> stats_rel \<rightarrow> stats_rel" 
+  "(add_lbd,add_lbd) \<in> word64_rel \<rightarrow> stats_rel \<rightarrow> stats_rel"
+  by auto
+
+
+  
+abbreviation (input) "restart_info_rel \<equiv> word64_rel \<times>\<^sub>r word64_rel"
+
+abbreviation (input) restart_info_assn where
+  \<open>restart_info_assn \<equiv> word64_assn *a word64_assn\<close>
+
+lemma restart_info_params[sepref_import_param]:  
+  "(incr_conflict_count_since_last_restart,incr_conflict_count_since_last_restart) \<in> restart_info_rel \<rightarrow> restart_info_rel"
+  "(restart_info_update_lvl_avg,restart_info_update_lvl_avg) \<in> word32_rel \<rightarrow> restart_info_rel \<rightarrow> restart_info_rel"
+  "(restart_info_init,restart_info_init) \<in> restart_info_rel"
+  "(restart_info_restart_done,restart_info_restart_done) \<in> restart_info_rel \<rightarrow> restart_info_rel"
+  by auto
+
+  
+type_synonym vmtf_node_assn = "(64 word \<times> 32 word \<times> 32 word)"    
+
+definition "vmtf_node1_rel \<equiv> { ((a,b,c),(VMTF_Node a b c)) | a b c. True}"
+definition "vmtf_node2_assn \<equiv> uint64_nat_assn *a snat_option_assn' TYPE(32) *a snat_option_assn' TYPE(32)"
+
+definition "vmtf_node_assn \<equiv> hr_comp vmtf_node2_assn vmtf_node1_rel"
+lemmas [fcomp_norm_unfold] = vmtf_node_assn_def[symmetric]
+
+lemma 
+    vmtf_Node_refine1: "(\<lambda>a b c. (a,b,c), VMTF_Node) \<in> Id \<rightarrow> Id \<rightarrow> Id \<rightarrow> vmtf_node1_rel"
+and vmtf_stamp_refine1: "(\<lambda>(a,b,c). a, stamp) \<in> vmtf_node1_rel \<rightarrow> Id"  
+and vmtf_get_prev_refine1: "(\<lambda>(a,b,c). b, get_prev) \<in> vmtf_node1_rel \<rightarrow> \<langle>Id\<rangle>option_rel"  
+and vmtf_get_next_refine1: "(\<lambda>(a,b,c). c, get_next) \<in> vmtf_node1_rel \<rightarrow> \<langle>Id\<rangle>option_rel"  
+  by (auto simp: vmtf_node1_rel_def)
+
+sepref_definition VMTF_Node_impl is "uncurry2 (RETURN ooo (\<lambda>a b c. (a,b,c)))" :: "uint64_nat_assn\<^sup>k *\<^sub>a (snat_option_assn' TYPE(32))\<^sup>k *\<^sub>a (snat_option_assn' TYPE(32))\<^sup>k \<rightarrow>\<^sub>a vmtf_node2_assn"
+  unfolding vmtf_node2_assn_def by sepref
+
+(* TODO: The below SHOULD work with RETURN o (\<lambda>(a,b,c). a), but this results in id-phase to fail! (probably already preproc-phase is botched! )*)  
+sepref_definition VMTF_stamp_impl is "(\<lambda>(a,b,c). RETURN a)" :: "vmtf_node2_assn\<^sup>k \<rightarrow>\<^sub>a uint64_nat_assn"
+  unfolding vmtf_node2_assn_def 
+  by sepref
+  
+sepref_definition VMTF_get_prev_impl is "(\<lambda>(a,b,c). RETURN b)" :: "vmtf_node2_assn\<^sup>k \<rightarrow>\<^sub>a snat_option_assn' TYPE(32)"
+  unfolding vmtf_node2_assn_def 
+  by sepref
+      
+sepref_definition VMTF_get_next_impl is "(\<lambda>(a,b,c). RETURN c)" :: "vmtf_node2_assn\<^sup>k \<rightarrow>\<^sub>a snat_option_assn' TYPE(32)"
+  unfolding vmtf_node2_assn_def 
+  by sepref
+
+lemma workaround_unfold_return_triple[fcomp_norm_unfold]: "(\<lambda>(a,b,c). RETURN (f a b c)) = RETURN o (\<lambda>(a,b,c). f a b c)" by auto
+  
+(* TODO: This should be done automatically! For all structured ID-relations on hr_comp! *)
+lemma workaround_hrcomp_id_norm[fcomp_norm_unfold]: "hr_comp R (\<langle>nat_rel\<rangle>option_rel) = R" by simp
+
+lemmas [sepref_fr_rules] = 
+  VMTF_Node_impl.refine[FCOMP vmtf_Node_refine1]  
+  VMTF_stamp_impl.refine[unfolded workaround_unfold_return_triple,FCOMP vmtf_stamp_refine1]
+  VMTF_get_prev_impl.refine[unfolded workaround_unfold_return_triple,FCOMP vmtf_get_prev_refine1]
+  VMTF_get_next_impl.refine[unfolded workaround_unfold_return_triple,FCOMP vmtf_get_next_refine1]
+  
+
+  
+    
+type_synonym vmtf_assn = \<open>vmtf_node_assn ptr \<times> 64 word \<times> 32 word \<times> 32 word \<times> 32 word\<close>  
+  
+type_synonym vmtf_remove_assn = \<open>vmtf_assn \<times> (32 word array_list32 \<times> 1 word ptr)\<close>
+
+
+abbreviation vmtf_assn :: "_ \<Rightarrow> vmtf_assn \<Rightarrow> assn" where
+  \<open>vmtf_assn \<equiv> (array_assn vmtf_node_assn *a uint64_nat_assn *a uint32_nat_assn *a uint32_nat_assn
+    *a snat_option_assn' TYPE(32))\<close>
+
+abbreviation atoms_hash_assn :: \<open>bool list \<Rightarrow> 1 word ptr \<Rightarrow> assn\<close> where
+  \<open>atoms_hash_assn \<equiv> array_assn bool1_assn\<close>
+
+abbreviation distinct_atoms_assn where
+  \<open>distinct_atoms_assn \<equiv> arl32_assn uint32_nat_assn *a atoms_hash_assn\<close>
+
+abbreviation vmtf_remove_assn
+  :: \<open>isa_vmtf_remove_int \<Rightarrow> vmtf_remove_assn \<Rightarrow> assn\<close>
+where
+  \<open>vmtf_remove_assn \<equiv> vmtf_assn *a distinct_atoms_assn\<close>
+
+
+paragraph \<open>Options\<close>
+
+type_synonym opts_assn = "1 word \<times> 1 word \<times> 1 word"
+
+abbreviation opts_assn
+  :: \<open>opts \<Rightarrow> opts_assn \<Rightarrow> assn\<close>
+where
+  \<open>opts_assn \<equiv> bool1_assn *a bool1_assn *a bool1_assn\<close>
+
+lemma workaround_opt_assn: "RETURN o (\<lambda>(a,b,c). f a b c) = (\<lambda>(a,b,c). RETURN (f a b c))" by auto
+
+sepref_register opts_restart opts_reduce opts_unbounded_mode
+  
+sepref_definition opts_restart_impl is "RETURN o opts_restart" :: "opts_assn\<^sup>k \<rightarrow>\<^sub>a bool1_assn"  
+  unfolding opts_restart_def workaround_opt_assn
+  by sepref
+
+sepref_definition opts_reduce_impl is "RETURN o opts_reduce" :: "opts_assn\<^sup>k \<rightarrow>\<^sub>a bool1_assn"  
+  unfolding opts_reduce_def workaround_opt_assn
+  by sepref
+
+sepref_definition opts_unbounded_mode_impl is "RETURN o opts_unbounded_mode" :: "opts_assn\<^sup>k \<rightarrow>\<^sub>a bool1_assn"  
+  unfolding opts_unbounded_mode_def workaround_opt_assn
+  by sepref
+  
+lemmas [sepref_fr_rules] = 
+  opts_restart_impl.refine
+  opts_reduce_impl.refine
+  opts_unbounded_mode_impl.refine
+  
+  
+abbreviation "watchlist_fast_assn \<equiv> aal_assn' TYPE(64) TYPE(64) watcher_fast_assn"
+
+
+type_synonym vdom_fast_assn = \<open>64 word array_list64\<close>
+abbreviation vdom_fast_assn :: \<open>vdom \<Rightarrow> vdom_fast_assn \<Rightarrow> assn\<close> where
+  \<open>vdom_fast_assn \<equiv> arl64_assn sint64_nat_assn\<close>
+
+type_synonym phase_saver_assn = "1 word larray32"
+abbreviation phase_saver_assn where
+  \<open>phase_saver_assn \<equiv> larray32_assn bool1_assn\<close>
+
+(* TODO: Move *)
+type_synonym arena_assn = "(32 word, 64) array_list"
+  
+typ "(32 word, 64) array_list"
+  
+type_synonym twl_st_wll_trail_fast =
+  \<open>trail_pol_fast_assn \<times> arena_assn \<times> option_lookup_clause_assn \<times>
+    32 word \<times> watched_wl_uint32 \<times> vmtf_remove_assn \<times> phase_saver_assn \<times>
+    32 word \<times> cach_refinement_l_assn \<times> lbd_assn \<times> out_learned_assn \<times> stats \<times> ema \<times> ema \<times> restart_info \<times>
+    vdom_fast_assn \<times> vdom_fast_assn \<times> 64 word \<times> opts_assn \<times> arena_assn\<close>
+
+
+definition isasat_bounded_assn :: \<open>twl_st_wl_heur \<Rightarrow> twl_st_wll_trail_fast \<Rightarrow> assn\<close> where
+\<open>isasat_bounded_assn =
+  trail_pol_fast_assn *a arena_fast_assn *a
+  conflict_option_rel_assn *a
+  uint32_nat_assn *a
+  watchlist_fast_assn *a
+  vmtf_remove_assn *a phase_saver_assn *a
+  uint32_nat_assn *a
+  cach_refinement_l_assn *a
+  lbd_assn *a
+  out_learned_assn *a
+  stats_assn *a
+  ema_assn *a
+  ema_assn *a
+  restart_info_assn *a
+  vdom_fast_assn *a
+  vdom_fast_assn *a
+  uint64_nat_assn *a
+  opts_assn *a arena_fast_assn\<close>
+
+
+subsubsection \<open>Lift Operations to State\<close>
+
+(*TODO proper setup to test if the conflict is none*)
+sepref_definition get_conflict_wl_is_None_fast_code
+  is \<open>RETURN o get_conflict_wl_is_None_heur\<close>
+  :: \<open>isasat_bounded_assn\<^sup>k \<rightarrow>\<^sub>a bool1_assn\<close>
+  unfolding get_conflict_wl_is_None_heur_alt_def isasat_bounded_assn_def length_ll_def[symmetric]
+    conflict_option_rel_assn_def
+  supply [[goals_limit=1]]
+  by sepref
+
+declare get_conflict_wl_is_None_fast_code.refine[sepref_fr_rules]
+
+sepref_definition isa_count_decided_st_fast_code
+  is \<open>RETURN o isa_count_decided_st\<close>
+  :: \<open>isasat_bounded_assn\<^sup>k \<rightarrow>\<^sub>a uint32_nat_assn\<close>
+  supply [[goals_limit=2]]
+  unfolding isa_count_decided_st_def isasat_bounded_assn_def
+  by sepref
+
+declare isa_count_decided_st_fast_code.refine[sepref_fr_rules]
+
+sepref_definition polarity_st_heur_pol_fast
+  is \<open>uncurry (RETURN oo polarity_st_heur)\<close>
+  :: \<open>[polarity_st_heur_pre]\<^sub>a isasat_bounded_assn\<^sup>k *\<^sub>a unat_lit_assn\<^sup>k \<rightarrow> tri_bool_assn\<close>
+  unfolding polarity_st_heur_alt_def isasat_bounded_assn_def polarity_st_pre_def
+    polarity_st_heur_pre_def
+  supply [[goals_limit = 1]]
+  by sepref
+
+declare polarity_st_heur_pol_fast.refine[sepref_fr_rules]
+
+
+subsection \<open>More theorems\<close>
+
+
+sepref_definition polarity_st_heur_pol_fast
+  is \<open>RETURN o count_decided_st_heur\<close>
+  :: \<open>isasat_bounded_assn\<^sup>k \<rightarrow>\<^sub>a uint32_nat_assn\<close>
+  unfolding isasat_bounded_assn_def count_decided_st_heur_def
+  supply [[goals_limit = 1]]
+  by sepref
+  
+  
+  
+lemma count_decided_st_heur[sepref_fr_rules]:
+  \<open>(return o count_decided_st_heur, RETURN o count_decided_st_heur) \<in>
+      isasat_bounded_assn\<^sup>k \<rightarrow>\<^sub>a uint32_nat_assn\<close>
+  unfolding count_decided_st_heur_def isasat_bounded_assn_def
+  apply sepref_to_hoare
+  apply vcg_normalize
+  apply (simp add: sep_algebra_simps pred_lift_extract_simps)
+  find_theorems "llvm_htriple (\<up>_ ** _)"
+  
+  by (sepref_to_hoare; sep_auto)+
+
+sepref_definition access_lit_in_clauses_heur_fast_code
+  is \<open>uncurry2 (RETURN ooo access_lit_in_clauses_heur)\<close>
+  :: \<open>[\<lambda>((S, i), j). access_lit_in_clauses_heur_pre ((S, i), j) \<and>
+           length (get_clauses_wl_heur S) \<le> sint64_max]\<^sub>a
+      isasat_bounded_assn\<^sup>k *\<^sub>a uint64_nat_assn\<^sup>k  *\<^sub>a uint64_nat_assn\<^sup>k \<rightarrow> unat_lit_assn\<close>
+  supply [[goals_limit=1]] arena_is_valid_clause_idx_le_uint64_max[intro]
+  unfolding isasat_bounded_assn_def access_lit_in_clauses_heur_alt_def
+    fmap_rll_def[symmetric] access_lit_in_clauses_heur_pre_def
+    fmap_rll_u64_def[symmetric] arena_lit_pre_le[intro]
+  by sepref
+
+declare access_lit_in_clauses_heur_fast_code.refine[sepref_fr_rules]
+
+sepref_register rewatch_heur
+sepref_definition rewatch_heur_fast_code
+  is \<open>uncurry2 (rewatch_heur)\<close>
+  :: \<open>[\<lambda>((vdom, arena), W). (\<forall>x \<in> set vdom. x \<le> uint64_max) \<and> length arena \<le> uint64_max \<and> length vdom \<le> sint64_max]\<^sub>a
+        vdom_fast_assn\<^sup>k *\<^sub>a arena_fast_assn\<^sup>k *\<^sub>a watchlist_fast_assn\<^sup>d \<rightarrow> watchlist_fast_assn\<close>
+  supply [[goals_limit=1]]
+     arena_lit_pre_le_uint64_max[intro]
+  unfolding rewatch_heur_alt_def Let_def PR_CONST_def
+  unfolding while_eq_nfoldli[symmetric]
+  apply (subst while_upt_while_direct, simp)
+  unfolding zero_uint64_nat_def[symmetric]
+    one_uint64_nat_def[symmetric] to_watcher_fast_def[symmetric]
+    FOREACH_cond_def FOREACH_body_def uint64_of_nat_conv_def
+  by sepref
+
+sepref_register append_ll
+
+declare rewatch_heur_fast_code.refine[sepref_fr_rules]
+
+
+sepref_definition rewatch_heur_st_fast_code
+  is \<open>(rewatch_heur_st_fast)\<close>
+  :: \<open>[rewatch_heur_st_fast_pre]\<^sub>a
+       isasat_bounded_assn\<^sup>d \<rightarrow> isasat_bounded_assn\<close>
+  supply [[goals_limit=1]]
+  unfolding rewatch_heur_st_def PR_CONST_def rewatch_heur_st_fast_pre_def
+    isasat_bounded_assn_def rewatch_heur_st_fast_def
+  by sepref
+
+declare rewatch_heur_st_code.refine[sepref_fr_rules]
+  rewatch_heur_st_fast_code.refine[sepref_fr_rules]
+
+end
