Weidenbach_Book/IsaSAT_Watch_List_LLVM.thy
@@ -3,7 +3,7 @@ theory IsaSAT_Watch_List_LLVM
 begin
 
 type_synonym watched_wl_uint32 
-  = \<open>(32,(64 word \<times> 32 word \<times> 1 word),64)array_array_list\<close>
+  = \<open>(64,(64 word \<times> 32 word \<times> 1 word),64)array_array_list\<close>
 
 abbreviation "watcher_fast_assn \<equiv> uint64_nat_assn *a unat_lit_assn *a bool1_assn   "
 
